refit term subst

Common/Term/Substitution.lean
@@ -16,17 +16,17 @@ end SubstAction
 
 def Subst (T : Type) : Type := Nat -> SubstAction T
 
-def subst_term_to_subst_cvterm : Subst Term -> Subst CvTerm
-| σ, n => match σ n with
-  | .rename k => .rename k
-  | .replace t => .replace (.refl t)
+-- def subst_term_to_subst_cvterm : Subst Term -> Subst CvTerm
+-- | σ, n => match σ n with
+--   | .rename k => .rename k
+--   | .replace t => .replace (.refl t)
 
-prefix:max "▸" => subst_term_to_subst_cvterm
+-- prefix:max "▸" => subst_term_to_subst_cvterm
 
-@[simp] def I : Ren := λ n => n
-@[simp] def S : Ren := λ n => n + 1
-@[simp] def Sn (x : Nat) : Ren := λ n => n + x
-@[simp] def Pn (x : Nat) : Ren := λ n => n - x
+@[simp] def rI : Ren := λ n => n
+@[simp] def rS : Ren := λ n => n + 1
+@[simp] def rSn (x : Nat) : Ren := λ n => n + x
+@[simp] def rPn (x : Nat) : Ren := λ n => n - x
 
 namespace Term
 
@@ -35,37 +35,37 @@ namespace Term
     | _, 0 => 0
     | σ, n + 1 => σ n + 1
 
-    @[simp]
-    def cvapply : Ren -> CvTerm -> CvTerm
-    | σ, .sym t => .sym (cvapply σ t)
-    | σ, .trans t1 t2 => .trans (cvapply σ t1) (cvapply σ t2)
-    | _, .none => .none
-    | _, .const => .const
-    | σ, .bound k => .bound (σ k)
-    | σ, .all_congr t1 t2 => .all_congr (cvapply σ t1) (cvapply (lift σ) t2)
-    | σ, .lam_congr t1 t2 => .lam_congr (cvapply σ t1) (cvapply (lift σ) t2)
-    | σ, .lam_eta t => .lam_eta (cvapply σ t)
-    | σ, .lam_mf_erased t => .lam_mf_erased (cvapply (lift σ) t)
-    | σ, .lam_m0_erased t => .lam_m0_erased (cvapply (lift σ) t)
-    | σ, .app_congr t1 t2 => .app_congr (cvapply σ t1) (cvapply σ t2)
-    | σ, .app_beta t => .app_beta (cvapply σ t)
-    | σ, .app_m0_erased t => .app_m0_erased (cvapply σ t)
-    | σ, .prod_congr t1 t2 => .prod_congr (cvapply σ t1) (cvapply (lift σ) t2)
-    | σ, .pair_congr t1 t2 t3 => .pair_congr (cvapply σ t1) (cvapply σ t2) (cvapply σ t3)
-    | σ, .pair_erased t => .pair_erased (cvapply σ t)
-    | σ, .fst_congr t => .fst_congr (cvapply σ t)
-    | σ, .fst_erased t => .fst_erased (cvapply σ t)
-    | σ, .snd_congr t => .snd_congr (cvapply σ t)
-    | σ, .snd_erased t => .snd_erased (cvapply σ t)
-    | σ, .phi_congr t1 t2 t3 => .phi_congr (cvapply σ t1) (cvapply σ t2) (cvapply σ t3)
-    | σ, .phi_erased t => .phi_erased (cvapply σ t)
-    | σ, .eq_congr t1 t2 t3 => .eq_congr (cvapply σ t1) (cvapply σ t2) (cvapply σ t3)
-    | σ, .refl_congr t => .refl_congr (cvapply σ t)
-    | σ, .refl_erased t => .refl_erased (cvapply σ t)
-    | σ, .subst_congr t1 t2 => .subst_congr (cvapply σ t1) (cvapply σ t2)
-    | σ, .subst_erased t => .subst_erased (cvapply σ t)
-    | σ, .conv_congr t1 t2 => .conv_congr (cvapply σ t1) (cvapply σ t2)
-    | σ, .conv_erased t => .conv_erased (cvapply σ t)
+    -- @[simp]
+    -- def cvapply : Ren -> CvTerm -> CvTerm
+    -- | σ, .sym t => .sym (cvapply σ t)
+    -- | σ, .trans t1 t2 => .trans (cvapply σ t1) (cvapply σ t2)
+    -- | _, .none => .none
+    -- | _, .const => .const
+    -- | σ, .bound k => .bound (σ k)
+    -- | σ, .all_congr t1 t2 => .all_congr (cvapply σ t1) (cvapply (lift σ) t2)
+    -- | σ, .lam_congr t1 t2 => .lam_congr (cvapply σ t1) (cvapply (lift σ) t2)
+    -- | σ, .lam_eta t => .lam_eta (cvapply σ t)
+    -- | σ, .lam_mf_erased t => .lam_mf_erased (cvapply (lift σ) t)
+    -- | σ, .lam_m0_erased t => .lam_m0_erased (cvapply (lift σ) t)
+    -- | σ, .app_congr t1 t2 => .app_congr (cvapply σ t1) (cvapply σ t2)
+    -- | σ, .app_beta t => .app_beta (cvapply σ t)
+    -- | σ, .app_m0_erased t => .app_m0_erased (cvapply σ t)
+    -- | σ, .prod_congr t1 t2 => .prod_congr (cvapply σ t1) (cvapply (lift σ) t2)
+    -- | σ, .pair_congr t1 t2 t3 => .pair_congr (cvapply σ t1) (cvapply σ t2) (cvapply σ t3)
+    -- | σ, .pair_erased t => .pair_erased (cvapply σ t)
+    -- | σ, .fst_congr t => .fst_congr (cvapply σ t)
+    -- | σ, .fst_erased t => .fst_erased (cvapply σ t)
+    -- | σ, .snd_congr t => .snd_congr (cvapply σ t)
+    -- | σ, .snd_erased t => .snd_erased (cvapply σ t)
+    -- | σ, .phi_congr t1 t2 t3 => .phi_congr (cvapply σ t1) (cvapply σ t2) (cvapply σ t3)
+    -- | σ, .phi_erased t => .phi_erased (cvapply σ t)
+    -- | σ, .eq_congr t1 t2 t3 => .eq_congr (cvapply σ t1) (cvapply σ t2) (cvapply σ t3)
+    -- | σ, .refl_congr t => .refl_congr (cvapply σ t)
+    -- | σ, .refl_erased t => .refl_erased (cvapply σ t)
+    -- | σ, .subst_congr t1 t2 => .subst_congr (cvapply σ t1) (cvapply σ t2)
+    -- | σ, .subst_erased t => .subst_erased (cvapply σ t)
+    -- | σ, .conv_congr t1 t2 => .conv_congr (cvapply σ t1) (cvapply σ t2)
+    -- | σ, .conv_erased t => .conv_erased (cvapply σ t)
 
     @[simp]
     def apply : Ren -> Term -> Term
@@ -83,7 +83,8 @@ namespace Term
     | σ, subst t1 t2 => subst (apply σ t1) (apply σ t2)
     | σ, phi t1 t2 t3 => phi (apply σ t1) (apply σ t2) (apply σ t3)
     | σ, eq t1 t2 t3 => eq (apply σ t1) (apply σ t2) (apply σ t3)
-    | σ, conv t1 t2 c => conv (apply σ t1) (apply σ t2) (cvapply σ c)
+    | σ, conv t1 t2 c => conv (apply σ t1) (apply σ t2) c
+    -- | σ, conv t1 t2 c => conv (apply σ t1) (apply σ t2) (cvapply σ c)
   end Ren
 
   namespace Subst
@@ -94,52 +95,52 @@ namespace Term
     | t, _, 0 => t
     | _, σ, n + 1 => σ n
 
-    def cvlift : Subst CvTerm -> Subst CvTerm
-    | _, 0 => .rename 0
-    | σ, n + 1 => match (σ n) with
-      | .replace t => .replace (Ren.cvapply S t)
-      | .rename k => .rename (S k)
+    -- def cvlift : Subst CvTerm -> Subst CvTerm
+    -- | _, 0 => .rename 0
+    -- | σ, n + 1 => match (σ n) with
+    --   | .replace t => .replace (Ren.cvapply rS t)
+    --   | .rename k => .rename (rS k)
 
     def lift : Subst Term -> Subst Term
     | _, 0 => .rename 0
     | σ, n + 1 => match (σ n) with
-      | .replace t => .replace (Ren.apply S t)
-      | .rename k => .rename (S k)
+      | .replace t => .replace (Ren.apply rS t)
+      | .rename k => .rename (rS k)
 
-    @[simp]
-    def cvapply : Subst CvTerm -> CvTerm -> CvTerm
-    | σ, .sym t => .sym (cvapply σ t)
-    | σ, .trans t1 t2 => .trans (cvapply σ t1) (cvapply σ t2)
-    | _, .none => .none
-    | _, .const => .const
-    | σ, .bound k =>
-      match σ k with
-      | .replace t => t
-      | .rename n => .bound n
-    | σ, .all_congr t1 t2 => .all_congr (cvapply σ t1) (cvapply (cvlift σ) t2)
-    | σ, .lam_congr t1 t2 => .lam_congr (cvapply σ t1) (cvapply (cvlift σ) t2)
-    | σ, .lam_eta t => .lam_eta (cvapply σ t)
-    | σ, .lam_mf_erased t => .lam_mf_erased (cvapply (cvlift σ) t)
-    | σ, .lam_m0_erased t => .lam_m0_erased (cvapply (cvlift σ) t)
-    | σ, .app_congr t1 t2 => .app_congr (cvapply σ t1) (cvapply σ t2)
-    | σ, .app_beta t => .app_beta (cvapply σ t)
-    | σ, .app_m0_erased t => .app_m0_erased (cvapply σ t)
-    | σ, .prod_congr t1 t2 => .prod_congr (cvapply σ t1) (cvapply (cvlift σ) t2)
-    | σ, .pair_congr t1 t2 t3 => .pair_congr (cvapply σ t1) (cvapply σ t2) (cvapply σ t3)
-    | σ, .pair_erased t => .pair_erased (cvapply σ t)
-    | σ, .fst_congr t => .fst_congr (cvapply σ t)
-    | σ, .fst_erased t => .fst_erased (cvapply σ t)
-    | σ, .snd_congr t => .snd_congr (cvapply σ t)
-    | σ, .snd_erased t => .snd_erased (cvapply σ t)
-    | σ, .phi_congr t1 t2 t3 => .phi_congr (cvapply σ t1) (cvapply σ t2) (cvapply σ t3)
-    | σ, .phi_erased t => .phi_erased (cvapply σ t)
-    | σ, .eq_congr t1 t2 t3 => .eq_congr (cvapply σ t1) (cvapply σ t2) (cvapply σ t3)
-    | σ, .refl_congr t => .refl_congr (cvapply σ t)
-    | σ, .refl_erased t => .refl_erased (cvapply σ t)
-    | σ, .subst_congr t1 t2 => .subst_congr (cvapply σ t1) (cvapply σ t2)
-    | σ, .subst_erased t => .subst_erased (cvapply σ t)
-    | σ, .conv_congr t1 t2 => .conv_congr (cvapply σ t1) (cvapply σ t2)
-    | σ, .conv_erased t => .conv_erased (cvapply σ t)
+    -- @[simp]
+    -- def cvapply : Subst CvTerm -> CvTerm -> CvTerm
+    -- | σ, .sym t => .sym (cvapply σ t)
+    -- | σ, .trans t1 t2 => .trans (cvapply σ t1) (cvapply σ t2)
+    -- | _, .none => .none
+    -- | _, .const => .const
+    -- | σ, .bound k =>
+    --   match σ k with
+    --   | .replace t => t
+    --   | .rename n => .bound n
+    -- | σ, .all_congr t1 t2 => .all_congr (cvapply σ t1) (cvapply (cvlift σ) t2)
+    -- | σ, .lam_congr t1 t2 => .lam_congr (cvapply σ t1) (cvapply (cvlift σ) t2)
+    -- | σ, .lam_eta t => .lam_eta (cvapply σ t)
+    -- | σ, .lam_mf_erased t => .lam_mf_erased (cvapply (cvlift σ) t)
+    -- | σ, .lam_m0_erased t => .lam_m0_erased (cvapply (cvlift σ) t)
+    -- | σ, .app_congr t1 t2 => .app_congr (cvapply σ t1) (cvapply σ t2)
+    -- | σ, .app_beta t => .app_beta (cvapply σ t)
+    -- | σ, .app_m0_erased t => .app_m0_erased (cvapply σ t)
+    -- | σ, .prod_congr t1 t2 => .prod_congr (cvapply σ t1) (cvapply (cvlift σ) t2)
+    -- | σ, .pair_congr t1 t2 t3 => .pair_congr (cvapply σ t1) (cvapply σ t2) (cvapply σ t3)
+    -- | σ, .pair_erased t => .pair_erased (cvapply σ t)
+    -- | σ, .fst_congr t => .fst_congr (cvapply σ t)
+    -- | σ, .fst_erased t => .fst_erased (cvapply σ t)
+    -- | σ, .snd_congr t => .snd_congr (cvapply σ t)
+    -- | σ, .snd_erased t => .snd_erased (cvapply σ t)
+    -- | σ, .phi_congr t1 t2 t3 => .phi_congr (cvapply σ t1) (cvapply σ t2) (cvapply σ t3)
+    -- | σ, .phi_erased t => .phi_erased (cvapply σ t)
+    -- | σ, .eq_congr t1 t2 t3 => .eq_congr (cvapply σ t1) (cvapply σ t2) (cvapply σ t3)
+    -- | σ, .refl_congr t => .refl_congr (cvapply σ t)
+    -- | σ, .refl_erased t => .refl_erased (cvapply σ t)
+    -- | σ, .subst_congr t1 t2 => .subst_congr (cvapply σ t1) (cvapply σ t2)
+    -- | σ, .subst_erased t => .subst_erased (cvapply σ t)
+    -- | σ, .conv_congr t1 t2 => .conv_congr (cvapply σ t1) (cvapply σ t2)
+    -- | σ, .conv_erased t => .conv_erased (cvapply σ t)
 
     @[simp]
     def apply : Subst Term -> Term -> Term
@@ -160,12 +161,13 @@ namespace Term
     | σ, subst t1 t2 => subst (apply σ t1) (apply σ t2)
     | σ, phi t1 t2 t3 => phi (apply σ t1) (apply σ t2) (apply σ t3)
     | σ, eq t1 t2 t3 => eq (apply σ t1) (apply σ t2) (apply σ t3)
-    | σ, conv t1 t2 c => conv (apply σ t1) (apply σ t2) (cvapply ▸σ c)
+    | σ, conv t1 t2 c => conv (apply σ t1) (apply σ t2) c
+    -- | σ, conv t1 t2 c => conv (apply σ t1) (apply σ t2) (cvapply ▸σ c)
 
-    def cvcompose : Subst CvTerm -> Subst CvTerm -> Subst CvTerm
-    | σ, τ, n => match (σ n) with
-      | .replace t => .replace (cvapply τ t)
-      | .rename k => τ k
+    -- def cvcompose : Subst CvTerm -> Subst CvTerm -> Subst CvTerm
+    -- | σ, τ, n => match (σ n) with
+    --   | .replace t => .replace (cvapply τ t)
+    --   | .rename k => τ k
 
     def compose : Subst Term -> Subst Term -> Subst Term
     | σ, τ, n => match (σ n) with
@@ -176,23 +178,25 @@ namespace Term
 
 end Term
 
+@[simp] def I : Subst Term := λ n => .rename n
+@[simp] def S : Subst Term := λ n => .rename (n + 1)
+@[simp] def Sn (x : Nat) : Subst Term := λ n => .rename (n + x)
+@[simp] def Pn (x : Nat) : Subst Term := λ n => .rename (n - x)
+
 @[simp]
 def beta : Term -> Subst Term
-| t => Term.Subst.cons (.replace t) (Term.Subst.from_ren I)
+| t => Term.Subst.cons (.replace t) I
 
--- notation:100 "r#" σ:110 => Subst.from_ren σ
 prefix:max "r#" => @Term.Subst.from_ren Term
-prefix:max "cr#" => @Term.Subst.from_ren CvTerm
--- notation:70 t:70 "::" σ:70 => Subst.cons t σ
+-- prefix:max "cr#" => @Term.Subst.from_ren CvTerm
 infix:70 "::" => Term.Subst.cons
---notation:100 "^" σ:110 => Subst.lift σ
 prefix:max "^" => Term.Subst.lift
 notation:1000 "^{" n "}" σ:90 => rep n Term.Subst.lift σ
-prefix:max "^" => Term.Subst.cvlift
+-- prefix:max "^" => Term.Subst.cvlift
 notation:90 "[" σ "]" t:89 => Term.Subst.apply σ t
-notation:90 "[" σ "]" t:89 => Term.Subst.cvapply σ t
+-- notation:90 "[" σ "]" t:89 => Term.Subst.cvapply σ t
 notation:90 τ:90 " ⊙ " σ:91 => Term.Subst.compose σ τ
-notation:90 τ:90 " ⊙ " σ:91 => Term.Subst.cvcompose σ τ
+-- notation:90 τ:90 " ⊙ " σ:91 => Term.Subst.cvcompose σ τ
 notation:90 s:90 "β[" t "]" => Term.Subst.apply (beta t) s
 
 namespace Term
@@ -200,8 +204,8 @@ namespace Term
   @[simp] theorem subst_from_ren_x : (r#r) x = .rename (r x) :=
     by unfold Subst.from_ren; rfl
 
-  @[simp] theorem subst_from_cvren_x : (cr#r) x = .rename (r x) :=
-    by unfold Subst.from_ren; rfl
+  -- @[simp] theorem subst_from_cvren_x : (cr#r) x = .rename (r x) :=
+  --   by unfold Subst.from_ren; rfl
 
   @[simp] theorem subst_cons_zero {σ : Subst T} : (s :: σ) 0 = s :=
     by unfold Subst.cons; rfl
@@ -224,35 +228,35 @@ namespace Term
       subst lhsdef; subst rhsdef; rfl
   }
 
-  @[simp]
-  theorem subst_cvlift_is_ren_cvlift r : cr#(Ren.lift r) = ^(cr#r) := by {
-    funext; case _ x =>
-    cases x
-    case zero =>
-      unfold Subst.from_ren; unfold Ren.lift; simp
-      unfold Subst.cvlift; simp
-    case _ n =>
-      generalize lhsdef : (r#(Ren.lift r)) (n + 1) = lhs
-      generalize rhsdef : (^(r#r)) (n + 1) = rhs
-      unfold Subst.from_ren at lhsdef; simp at *
-      unfold Ren.lift at lhsdef; simp at *
-      unfold Subst.lift at rhsdef; simp at *
-      subst lhsdef; subst rhsdef; rfl
-  }
+  -- @[simp]
+  -- theorem subst_cvlift_is_ren_cvlift r : cr#(Ren.lift r) = ^(cr#r) := by {
+  --   funext; case _ x =>
+  --   cases x
+  --   case zero =>
+  --     unfold Subst.from_ren; unfold Ren.lift; simp
+  --     unfold Subst.cvlift; simp
+  --   case _ n =>
+  --     generalize lhsdef : (r#(Ren.lift r)) (n + 1) = lhs
+  --     generalize rhsdef : (^(r#r)) (n + 1) = rhs
+  --     unfold Subst.from_ren at lhsdef; simp at *
+  --     unfold Ren.lift at lhsdef; simp at *
+  --     unfold Subst.lift at rhsdef; simp at *
+  --     subst lhsdef; subst rhsdef; rfl
+  -- }
 
-  @[simp]
-  theorem subst_cvapply_is_ren_cvapply r t : Ren.cvapply r t = [cr#r]t := by {
-    induction t generalizing r
-    any_goals (unfold Ren.cvapply; simp [*])
-  }
+  -- @[simp]
+  -- theorem subst_cvapply_is_ren_cvapply r t : Ren.cvapply r t = [cr#r]t := by {
+  --   induction t generalizing r
+  --   any_goals (unfold Ren.cvapply; simp [*])
+  -- }
 
-  @[simp]
-  theorem subst_from_ren_transport_is_same : ▸(r#r) = cr#r := by {
-    funext
-    case _ x =>
-      cases x
-      all_goals (unfold Subst.from_ren; unfold subst_term_to_subst_cvterm; simp [*])
-  }
+  -- @[simp]
+  -- theorem subst_from_ren_transport_is_same : ▸(r#r) = cr#r := by {
+  --   funext
+  --   case _ x =>
+  --     cases x
+  --     all_goals (unfold Subst.from_ren; unfold subst_term_to_subst_cvterm; simp [*])
+  -- }
 
   @[simp]
   theorem subst_apply_is_ren_apply r t : Ren.apply r t = [r#r]t := by {
@@ -260,25 +264,28 @@ namespace Term
     any_goals (unfold Ren.apply; simp [*])
   }
 
-  @[simp]
-  theorem subst_cvapply_I_is_id s : [cr#I]s = s := by {
-    have lem : ^(cr# I) = cr# I := by {
-      funext
-      case _ x =>
-      cases x
-      case _ =>
-        unfold Subst.cvlift; simp
-      case _ x =>
-        unfold Subst.cvlift; simp
-    }
-    induction s
-    all_goals unfold Subst.cvapply
-    any_goals simp [*]
-  }
+  -- @[simp]
+  -- theorem subst_cvapply_I_is_id s : [cr#rI]s = s := by {
+  --   have lem : ^(cr# rI) = cr# rI := by {
+  --     funext
+  --     case _ x =>
+  --     cases x
+  --     case _ =>
+  --       unfold Subst.cvlift; simp
+  --     case _ x =>
+  --       unfold Subst.cvlift; simp
+  --   }
+  --   induction s
+  --   all_goals unfold Subst.cvapply
+  --   any_goals simp [*]
+  -- }
+
+  -- @[simp]
+  -- theorem subst_transform_subst_I_is_crI : ▸I = cr#rI := by sorry
 
   @[simp]
-  theorem subst_apply_I_is_id s : [r#I]s = s := by {
-    have lem : ^(r# I) = r# I := by {
+  theorem subst_apply_I_is_id {s : Term} : [I]s = s := by {
+    have lem : ^I = I := by {
       funext
       case _ x =>
       cases x
@@ -292,174 +299,174 @@ namespace Term
     any_goals simp [*]
   }
 
-  theorem subst_transform_ren_apply_commutes : .refl ([r#r]t) = [cr#r] (.refl t) := by {
-    induction t generalizing r
-    all_goals simp [*]
-    case lam m t1 t2 ih1 ih2 => rw [<-subst_cvlift_is_ren_cvlift, <-subst_lift_is_ren_lift, ih2]
-    case all m t1 t2 ih1 ih2 => rw [<-subst_cvlift_is_ren_cvlift, <-subst_lift_is_ren_lift, ih2]
-    case prod t1 t2 ih1 ih2 => rw [<-subst_cvlift_is_ren_cvlift, <-subst_lift_is_ren_lift, ih2]
-  }
+  -- theorem subst_transform_ren_apply_commutes : .refl ([r#r]t) = [cr#r] (.refl t) := by {
+  --   induction t generalizing r
+  --   all_goals simp [*]
+  --   case lam m t1 t2 ih1 ih2 => rw [<-subst_cvlift_is_ren_cvlift, <-subst_lift_is_ren_lift, ih2]
+  --   case all m t1 t2 ih1 ih2 => rw [<-subst_cvlift_is_ren_cvlift, <-subst_lift_is_ren_lift, ih2]
+  --   case prod t1 t2 ih1 ih2 => rw [<-subst_cvlift_is_ren_cvlift, <-subst_lift_is_ren_lift, ih2]
+  -- }
 
-  @[simp]
-  theorem subst_transform_lift_commutes : ▸^σ = ^▸σ := by {
-    funext
-    case _ x =>
-    unfold subst_term_to_subst_cvterm; unfold Subst.lift; unfold Subst.cvlift; simp
-    cases x
-    case _ => simp
-    case _ n =>
-      simp
-      cases σ n
-      case _ => simp
-      case _ t =>
-        simp; rw [subst_transform_ren_apply_commutes]
-  }
+  -- @[simp]
+  -- theorem subst_transform_lift_commutes : ▸^σ = ^▸σ := by {
+  --   funext
+  --   case _ x =>
+  --   unfold subst_term_to_subst_cvterm; unfold Subst.lift; unfold Subst.cvlift; simp
+  --   cases x
+  --   case _ => simp
+  --   case _ n =>
+  --     simp
+  --     cases σ n
+  --     case _ => simp
+  --     case _ t =>
+  --       simp; rw [subst_transform_ren_apply_commutes]
+  -- }
 
-  theorem subst_transform_apply_commutes : .refl ([σ]t) = [▸σ](.refl t) := by {
-    induction t generalizing σ
-    all_goals simp [*]
-    case bound k i =>
-      unfold subst_term_to_subst_cvterm; simp
-      cases σ i
-      case _ j => simp
-      case _ s => simp
-  }
+  -- theorem subst_transform_apply_commutes : .refl ([σ]t) = [▸σ](.refl t) := by {
+  --   induction t generalizing σ
+  --   all_goals simp [*]
+  --   case bound k i =>
+  --     unfold subst_term_to_subst_cvterm; simp
+  --     cases σ i
+  --     case _ j => simp
+  --     case _ s => simp
+  -- }
 
-  @[simp]
-  theorem subst_transform_commutes_with_compose : ▸(σ ⊙ τ) = ▸σ ⊙ ▸τ := by {
-    funext
-    case _ x =>
-    unfold subst_term_to_subst_cvterm; unfold Subst.compose; unfold Subst.cvcompose; simp
-    cases (τ x)
-    case _ x => simp
-    case _ t =>
-      simp; rw [subst_transform_apply_commutes]
-      unfold subst_term_to_subst_cvterm; simp
-  }
+  -- @[simp]
+  -- theorem subst_transform_commutes_with_compose : ▸(σ ⊙ τ) = ▸σ ⊙ ▸τ := by {
+  --   funext
+  --   case _ x =>
+  --   unfold subst_term_to_subst_cvterm; unfold Subst.compose; unfold Subst.cvcompose; simp
+  --   cases (τ x)
+  --   case _ x => simp
+  --   case _ t =>
+  --     simp; rw [subst_transform_apply_commutes]
+  --     unfold subst_term_to_subst_cvterm; simp
+  -- }
 
-  @[simp]
-  theorem subst_transform_commutes_with_cons_rename : ▸(.rename k :: σ) = .rename k :: ▸σ := by {
-    funext
-    case _ x =>
-      unfold subst_term_to_subst_cvterm
-      cases x <;> simp [*]
-  }
+  -- @[simp]
+  -- theorem subst_transform_commutes_with_cons_rename : ▸(.rename k :: σ) = .rename k :: ▸σ := by {
+  --   funext
+  --   case _ x =>
+  --     unfold subst_term_to_subst_cvterm
+  --     cases x <;> simp [*]
+  -- }
 
-  @[simp]
-  theorem subst_transform_commutes_with_cons_replace : ▸(.replace t :: σ) = .replace (.refl t) :: ▸σ := by {
-    funext
-    case _ x =>
-      unfold subst_term_to_subst_cvterm
-      cases x <;> simp [*]
-  }
+  -- @[simp]
+  -- theorem subst_transform_commutes_with_cons_replace : ▸(.replace t :: σ) = .replace (.refl t) :: ▸σ := by {
+  --   funext
+  --   case _ x =>
+  --     unfold subst_term_to_subst_cvterm
+  --     cases x <;> simp [*]
+  -- }
 
-  @[simp]
-  theorem subst_cvapply_twice_is_cvapply_compose {s : CvTerm} {σ τ} : [τ][σ]s = [τ ⊙ σ]s := by {
-    have lem1 τ : ^τ ⊙ cr#S = cr#S ⊙ τ := by {
-      funext
-      unfold Subst.cvcompose; unfold Subst.from_ren; unfold S; simp
-      unfold Subst.cvlift; unfold S; simp
-      unfold Subst.from_ren; simp
-    }
-    have lem2 (σ:Subst CvTerm) e : ^(σ ⊙ cr#e) = ^σ ⊙ ^(cr#e) := by {
-      funext; case _ n =>
-      cases n
-      . unfold Subst.from_ren; unfold Subst.cvcompose; unfold Subst.cvlift; simp
-      case _ n =>
-        generalize lhsdef : (^σ ⊙ ^(cr#e)) (n + 1) = lhs
-        unfold Subst.cvlift; simp
-        unfold Subst.cvcompose; unfold Subst.from_ren; unfold S; simp
-        subst lhs; unfold Subst.cvcompose; unfold Subst.cvlift; simp
-        unfold Subst.from_ren; unfold S; simp
-    }
-    have lem3 σ e s : [σ][cr#e]s = [σ ⊙ cr#e]s := by {
-      induction s generalizing σ e
-      any_goals simp [*]
-      case bound => unfold Subst.cvcompose; simp
-      case all_congr _ _ _ ih => rw [<-subst_cvlift_is_ren_cvlift, ih]
-      case lam_congr _ _ _ ih => rw [<-subst_cvlift_is_ren_cvlift, ih]
-      case lam_mf_erased _ ih => rw [<-subst_cvlift_is_ren_cvlift, ih]
-      case lam_m0_erased _ ih => rw [<-subst_cvlift_is_ren_cvlift, ih]
-      case prod_congr _ _ _ ih => rw [<-subst_cvlift_is_ren_cvlift, ih]
-    }
-    have lem4 σ τ : σ ⊙ τ ⊙ cr#S = σ ⊙ (τ ⊙ cr#S) := by {
-      funext; case _ x =>
-      cases x
-      any_goals (unfold Subst.cvcompose; unfold Subst.from_ren; unfold S; simp)
-    }
-    have lem5 r1 r2 τ : cr#r1 ⊙ (cr#r2 ⊙ τ) = cr#r1 ⊙ cr#r2 ⊙ τ := by {
-      funext; case _ x =>
-        unfold Subst.cvcompose; simp
-        cases τ x <;> simp at *
-        case _ t =>
-          have lem : [fun x => SubstAction.rename (r1 (r2 x))]t = [cr#r1 ⊙ cr#r2]t := by {
-            unfold Subst.cvcompose; simp
-          }
-          rw [lem, lem3]
-    }
-    have lem6 e τ : ^(cr#e) ⊙ ^τ = ^(cr#e ⊙ τ) := by {
-      funext; case _ n =>
-      cases n
-      . unfold Subst.cvcompose; unfold Subst.cvlift; simp
-      case _ n =>
-        have lem : ((^(cr#e) ⊙ ^τ) ⊙ cr#S) n = (^(cr#e ⊙ τ) ⊙ cr#S) n := by {
-          rw [lem1, lem4, lem1]
-          rw [<-subst_cvlift_is_ren_cvlift, lem5]; simp
-          rw [lem1, lem5]
-        }
-        unfold Subst.cvcompose at lem; unfold S at lem; unfold Subst.from_ren at lem
-        unfold Subst.cvcompose; unfold Subst.from_ren
-        simp at lem; simp [*]
-    }
-    have lem7 τ e s : [cr#e][τ]s = [cr#e ⊙ τ]s := by {
-      induction s generalizing τ e
-      any_goals simp [*]
-      case bound k =>
-        unfold Subst.cvcompose; simp
-        cases τ k <;> simp at *
-      case all_congr _ _ _ ih => rw [<-subst_cvlift_is_ren_cvlift, ih, <-lem6]; simp
-      case lam_congr _ _ _ ih => rw [<-subst_cvlift_is_ren_cvlift, ih, <-lem6]; simp
-      case lam_mf_erased _ ih => rw [<-subst_cvlift_is_ren_cvlift, ih, <-lem6]; simp
-      case lam_m0_erased _ ih => rw [<-subst_cvlift_is_ren_cvlift, ih, <-lem6]; simp
-      case prod_congr _ _ _ ih => rw [<-subst_cvlift_is_ren_cvlift, ih, <-lem6]; simp
-    }
-    have lem8 σ τ : σ ⊙ (cr#S ⊙ τ) = σ ⊙ cr#S ⊙ τ := by {
-      funext; case _ x =>
-        unfold Subst.cvcompose; simp
-        cases τ x <;> simp at *
-        rw [lem3]; unfold Subst.cvcompose; simp
-    }
-    have lem9 σ τ : cr#S ⊙ (σ ⊙ τ) = cr#S ⊙ σ ⊙ τ := by {
-      funext; case _ x =>
-        unfold Subst.cvcompose; simp
-        cases τ x <;> simp at *
-        rw [lem7]; unfold Subst.cvcompose; simp
-    }
-    have lem10 (σ τ : Subst CvTerm) : ^σ ⊙ ^τ = ^(σ ⊙ τ) := by {
-      funext; case _ x =>
-      cases x
-      case _ => unfold Subst.cvcompose; unfold Subst.cvlift; simp
-      case _ n =>
-        have lem : ((^σ ⊙ ^τ) ⊙ cr#S) n = (^(σ ⊙ τ) ⊙ cr#S) n := by {
-          rw [lem1, lem4, lem1, lem8, lem1, lem9]
-        }
-        unfold Subst.cvcompose at lem; unfold S at lem; unfold Subst.from_ren at lem
-        unfold Subst.cvcompose
-        simp at lem; simp [*]
-    }
-    induction s generalizing τ σ
-    any_goals simp [*]
-    case bound k =>
-      unfold Subst.cvcompose; simp
-      cases σ k <;> simp
-  }
+  -- @[simp]
+  -- theorem subst_cvapply_twice_is_cvapply_compose {s : CvTerm} {σ τ} : [τ][σ]s = [τ ⊙ σ]s := by {
+  --   have lem1 τ : ^τ ⊙ cr#rS = cr#rS ⊙ τ := by {
+  --     funext
+  --     unfold Subst.cvcompose; unfold Subst.from_ren; unfold rS; simp
+  --     unfold Subst.cvlift; unfold rS; simp
+  --     unfold Subst.from_ren; simp
+  --   }
+  --   have lem2 (σ:Subst CvTerm) e : ^(σ ⊙ cr#e) = ^σ ⊙ ^(cr#e) := by {
+  --     funext; case _ n =>
+  --     cases n
+  --     . unfold Subst.from_ren; unfold Subst.cvcompose; unfold Subst.cvlift; simp
+  --     case _ n =>
+  --       generalize lhsdef : (^σ ⊙ ^(cr#e)) (n + 1) = lhs
+  --       unfold Subst.cvlift; simp
+  --       unfold Subst.cvcompose; unfold Subst.from_ren; unfold rS; simp
+  --       subst lhs; unfold Subst.cvcompose; unfold Subst.cvlift; simp
+  --       unfold Subst.from_ren; unfold rS; simp
+  --   }
+  --   have lem3 σ e s : [σ][cr#e]s = [σ ⊙ cr#e]s := by {
+  --     induction s generalizing σ e
+  --     any_goals simp [*]
+  --     case bound => unfold Subst.cvcompose; simp
+  --     case all_congr _ _ _ ih => rw [<-subst_cvlift_is_ren_cvlift, ih]
+  --     case lam_congr _ _ _ ih => rw [<-subst_cvlift_is_ren_cvlift, ih]
+  --     case lam_mf_erased _ ih => rw [<-subst_cvlift_is_ren_cvlift, ih]
+  --     case lam_m0_erased _ ih => rw [<-subst_cvlift_is_ren_cvlift, ih]
+  --     case prod_congr _ _ _ ih => rw [<-subst_cvlift_is_ren_cvlift, ih]
+  --   }
+  --   have lem4 σ τ : σ ⊙ τ ⊙ cr#rS = σ ⊙ (τ ⊙ cr#rS) := by {
+  --     funext; case _ x =>
+  --     cases x
+  --     any_goals (unfold Subst.cvcompose; unfold Subst.from_ren; unfold rS; simp)
+  --   }
+  --   have lem5 r1 r2 τ : cr#r1 ⊙ (cr#r2 ⊙ τ) = cr#r1 ⊙ cr#r2 ⊙ τ := by {
+  --     funext; case _ x =>
+  --       unfold Subst.cvcompose; simp
+  --       cases τ x <;> simp at *
+  --       case _ t =>
+  --         have lem : [fun x => SubstAction.rename (r1 (r2 x))]t = [cr#r1 ⊙ cr#r2]t := by {
+  --           unfold Subst.cvcompose; simp
+  --         }
+  --         rw [lem, lem3]
+  --   }
+  --   have lem6 e τ : ^(cr#e) ⊙ ^τ = ^(cr#e ⊙ τ) := by {
+  --     funext; case _ n =>
+  --     cases n
+  --     . unfold Subst.cvcompose; unfold Subst.cvlift; simp
+  --     case _ n =>
+  --       have lem : ((^(cr#e) ⊙ ^τ) ⊙ cr#rS) n = (^(cr#e ⊙ τ) ⊙ cr#rS) n := by {
+  --         rw [lem1, lem4, lem1]
+  --         rw [<-subst_cvlift_is_ren_cvlift, lem5]; simp
+  --         rw [lem1, lem5]
+  --       }
+  --       unfold Subst.cvcompose at lem; unfold rS at lem; unfold Subst.from_ren at lem
+  --       unfold Subst.cvcompose; unfold Subst.from_ren
+  --       simp at lem; simp [*]
+  --   }
+  --   have lem7 τ e s : [cr#e][τ]s = [cr#e ⊙ τ]s := by {
+  --     induction s generalizing τ e
+  --     any_goals simp [*]
+  --     case bound k =>
+  --       unfold Subst.cvcompose; simp
+  --       cases τ k <;> simp at *
+  --     case all_congr _ _ _ ih => rw [<-subst_cvlift_is_ren_cvlift, ih, <-lem6]; simp
+  --     case lam_congr _ _ _ ih => rw [<-subst_cvlift_is_ren_cvlift, ih, <-lem6]; simp
+  --     case lam_mf_erased _ ih => rw [<-subst_cvlift_is_ren_cvlift, ih, <-lem6]; simp
+  --     case lam_m0_erased _ ih => rw [<-subst_cvlift_is_ren_cvlift, ih, <-lem6]; simp
+  --     case prod_congr _ _ _ ih => rw [<-subst_cvlift_is_ren_cvlift, ih, <-lem6]; simp
+  --   }
+  --   have lem8 σ τ : σ ⊙ (cr#rS ⊙ τ) = σ ⊙ cr#rS ⊙ τ := by {
+  --     funext; case _ x =>
+  --       unfold Subst.cvcompose; simp
+  --       cases τ x <;> simp at *
+  --       rw [lem3]; unfold Subst.cvcompose; simp
+  --   }
+  --   have lem9 σ τ : cr#rS ⊙ (σ ⊙ τ) = cr#rS ⊙ σ ⊙ τ := by {
+  --     funext; case _ x =>
+  --       unfold Subst.cvcompose; simp
+  --       cases τ x <;> simp at *
+  --       rw [lem7]; unfold Subst.cvcompose; simp
+  --   }
+  --   have lem10 (σ τ : Subst CvTerm) : ^σ ⊙ ^τ = ^(σ ⊙ τ) := by {
+  --     funext; case _ x =>
+  --     cases x
+  --     case _ => unfold Subst.cvcompose; unfold Subst.cvlift; simp
+  --     case _ n =>
+  --       have lem : ((^σ ⊙ ^τ) ⊙ cr#rS) n = (^(σ ⊙ τ) ⊙ cr#rS) n := by {
+  --         rw [lem1, lem4, lem1, lem8, lem1, lem9]
+  --       }
+  --       unfold Subst.cvcompose at lem; unfold rS at lem; unfold Subst.from_ren at lem
+  --       unfold Subst.cvcompose
+  --       simp at lem; simp [*]
+  --   }
+  --   induction s generalizing τ σ
+  --   any_goals simp [*]
+  --   case bound k =>
+  --     unfold Subst.cvcompose; simp
+  --     cases σ k <;> simp
+  -- }
 
   @[simp]
   theorem subst_apply_twice_is_apply_compose {s : Term} {σ τ} : [τ][σ]s = [τ ⊙ σ]s := by {
-    have lem1 τ : ^τ ⊙ r#S = r#S ⊙ τ := by {
+    have lem1 τ : ^τ ⊙ r#rS = r#rS ⊙ τ := by {
       funext
-      unfold Subst.compose; unfold Subst.from_ren; unfold S; simp
-      unfold Subst.lift; unfold S; simp
+      unfold Subst.compose; unfold Subst.from_ren; unfold rS; simp
+      unfold Subst.lift; unfold rS; simp
       unfold Subst.from_ren; simp
     }
     have lem2 (σ:Subst Term) e : ^(σ ⊙ r#e) = ^σ ⊙ ^(r#e) := by {
@@ -469,9 +476,9 @@ namespace Term
       case _ n =>
         generalize lhsdef : (^σ ⊙ ^(r#e)) (n + 1) = lhs
         unfold Subst.lift; simp
-        unfold Subst.compose; unfold Subst.from_ren; unfold S; simp
+        unfold Subst.compose; unfold Subst.from_ren; unfold rS; simp
         subst lhs; unfold Subst.compose; unfold Subst.lift; simp
-        unfold Subst.from_ren; unfold S; simp
+        unfold Subst.from_ren; unfold rS; simp
     }
     have lem3 σ e s : [σ][r#e]s = [σ ⊙ r#e]s := by {
       induction s generalizing σ e
@@ -481,10 +488,10 @@ namespace Term
       case all _ _ _ ih => rw [<-subst_lift_is_ren_lift, ih]
       case prod _ _ _ ih => rw [<-subst_lift_is_ren_lift, ih]
     }
-    have lem4 σ τ : σ ⊙ τ ⊙ r#S = σ ⊙ (τ ⊙ r#S) := by {
+    have lem4 σ τ : σ ⊙ τ ⊙ r#rS = σ ⊙ (τ ⊙ r#rS) := by {
       funext; case _ x =>
       cases x
-      any_goals (unfold Subst.compose; unfold Subst.from_ren; unfold S; simp)
+      any_goals (unfold Subst.compose; unfold Subst.from_ren; unfold rS; simp)
     }
     have lem5 r1 r2 τ : r#r1 ⊙ (r#r2 ⊙ τ) = r#r1 ⊙ r#r2 ⊙ τ := by {
       funext; case _ x =>
@@ -501,12 +508,12 @@ namespace Term
       cases n
       . unfold Subst.compose; unfold Subst.lift; simp
       case _ n =>
-        have lem : ((^(r#e) ⊙ ^τ) ⊙ r#S) n = (^(r#e ⊙ τ) ⊙ r#S) n := by {
+        have lem : ((^(r#e) ⊙ ^τ) ⊙ r#rS) n = (^(r#e ⊙ τ) ⊙ r#rS) n := by {
           rw [lem1, lem4, lem1]
           rw [<-subst_lift_is_ren_lift, lem5]; simp
           rw [lem1, lem5]
         }
-        unfold Subst.compose at lem; unfold S at lem; unfold Subst.from_ren at lem
+        unfold Subst.compose at lem; unfold rS at lem; unfold Subst.from_ren at lem
         unfold Subst.compose; unfold Subst.from_ren
         simp at lem; simp [*]
     }
@@ -520,13 +527,13 @@ namespace Term
       case all _ _ _ ih => rw [<-subst_lift_is_ren_lift, ih, <-lem6]; simp
       case prod _ _ _ ih => rw [<-subst_lift_is_ren_lift, ih, <-lem6]; simp
     }
-    have lem8 σ τ : σ ⊙ (r#S ⊙ τ) = σ ⊙ r#S ⊙ τ := by {
+    have lem8 σ τ : σ ⊙ (r#rS ⊙ τ) = σ ⊙ r#rS ⊙ τ := by {
       funext; case _ x =>
         unfold Subst.compose; simp
         cases τ x <;> simp at *
         rw [lem3]; unfold Subst.compose; simp
     }
-    have lem9 σ τ : r#S ⊙ (σ ⊙ τ) = r#S ⊙ σ ⊙ τ := by {
+    have lem9 σ τ : r#rS ⊙ (σ ⊙ τ) = r#rS ⊙ σ ⊙ τ := by {
       funext; case _ x =>
         unfold Subst.compose; simp
         cases τ x <;> simp at *
@@ -537,10 +544,10 @@ namespace Term
       cases x
       case _ => unfold Subst.compose; unfold Subst.lift; simp
       case _ n =>
-        have lem : ((^σ ⊙ ^τ) ⊙ r#S) n = (^(σ ⊙ τ) ⊙ r#S) n := by {
+        have lem : ((^σ ⊙ ^τ) ⊙ r#rS) n = (^(σ ⊙ τ) ⊙ r#rS) n := by {
           rw [lem1, lem4, lem1, lem8, lem1, lem9]
         }
-        unfold Subst.compose at lem; unfold S at lem; unfold Subst.from_ren at lem
+        unfold Subst.compose at lem; unfold rS at lem; unfold Subst.from_ren at lem
         unfold Subst.compose
         simp at lem; simp [*]
     }
@@ -552,7 +559,7 @@ namespace Term
   }
 
 
-  theorem subst_valid1 : s β[t] = [.replace t :: r#I]s
+  theorem subst_valid1 : s β[t] = [.replace t :: I]s
   := by simp
 
   @[simp] -- 0[s.σ ] = s
@@ -565,70 +572,72 @@ namespace Term
     : [.rename k :: σ]bound c 0 = bound c k
   := by unfold Subst.cons; simp
 
-  @[simp]
-  theorem cvsubst_valid2_replace
-    : [.replace s :: σ]CvTerm.bound 0 = s
-  := by unfold Subst.cons; simp
+  -- @[simp]
+  -- theorem cvsubst_valid2_replace
+  --   : [.replace s :: σ]CvTerm.bound 0 = s
+  -- := by unfold Subst.cons; simp
 
-  @[simp]
-  theorem cvsubst_valid2_rename
-    : [.rename k :: σ]CvTerm.bound 0 = CvTerm.bound k
-  := by unfold Subst.cons; simp
+  -- @[simp]
+  -- theorem cvsubst_valid2_rename
+  --   : [.rename k :: σ]CvTerm.bound 0 = CvTerm.bound k
+  -- := by unfold Subst.cons; simp
 
   @[simp] -- ⇑σ = 0.(σ ◦ S)
-  theorem subst_valid3 {σ : Subst Term} : ^σ = .rename 0 :: (r#S ⊙ σ) := by {
+  theorem subst_valid3 {σ : Subst Term} : ^σ = .rename 0 :: (S ⊙ σ) := by {
     funext; case _ x =>
       unfold Subst.lift; simp
       unfold Subst.compose; simp
+      unfold S; unfold Subst.from_ren; simp
       cases x
       case _ => simp
       case _ n => simp
   }
 
-  @[simp]
-  theorem cvsubst_valid3 {σ : Subst CvTerm} : ^σ = .rename 0 :: (cr#S ⊙ σ) := by {
-    funext; case _ x =>
-      unfold Subst.cvlift; simp
-      unfold Subst.cvcompose; simp
-      cases x
-      case _ => simp
-      case _ n => simp
-  }
+  -- @[simp]
+  -- theorem cvsubst_valid3 {σ : Subst CvTerm} : ^σ = .rename 0 :: (S ⊙ σ) := by {
+  --   funext; case _ x =>
+  --     unfold Subst.cvlift; simp
+  --     unfold Subst.cvcompose; simp
+  --     unfold S; unfold Subst.from_ren; simp
+  --     cases x
+  --     case _ => simp
+  --     case _ n => simp
+  -- }
 
   @[simp] -- 0.S = I
-  theorem subst_valid4 : .rename 0 :: r#S = r#I := by {
+  theorem subst_valid4 : .rename 0 :: S = I := by {
     funext; case _ x =>
     cases x
     case _ =>
-      unfold Subst.cons; unfold Subst.from_ren; simp
+      unfold Subst.cons; unfold S; simp
     case _ n =>
-      unfold Subst.cons; unfold Subst.from_ren; simp
+      unfold Subst.cons; unfold S; simp
   }
 
-  @[simp]
-  theorem cvsubst_valid4 : .rename 0 :: cr#S = cr#I := by {
-    funext; case _ x =>
-    cases x
-    case _ =>
-      unfold Subst.cons; unfold Subst.from_ren; simp
-    case _ n =>
-      unfold Subst.cons; unfold Subst.from_ren; simp
-  }
+  -- @[simp]
+  -- theorem cvsubst_valid4 : .rename 0 :: S = @I CvTerm := by {
+  --   funext; case _ x =>
+  --   cases x
+  --   case _ =>
+  --     unfold Subst.cons; unfold S; simp
+  --   case _ n =>
+  --     unfold Subst.cons; unfold S; simp
+  -- }
 
   @[simp] -- σ ◦ I = σ
-  theorem subst_valid5 : σ ⊙ r#I = σ := by {
+  theorem subst_valid5 {σ : Subst Term} : σ ⊙ I = σ := by {
     funext; case _ x =>
-    unfold Subst.compose; unfold Subst.from_ren; unfold I; simp
+    unfold Subst.compose; unfold I; simp
   }
 
-  @[simp]
-  theorem cvsubst_valid5 : σ ⊙ cr#I = σ := by {
-    funext; case _ x =>
-    unfold Subst.cvcompose; unfold Subst.from_ren; unfold I; simp
-  }
+  -- @[simp]
+  -- theorem cvsubst_valid5 {σ : Subst CvTerm} : σ ⊙ I = σ := by {
+  --   funext; case _ x =>
+  --   unfold Subst.cvcompose; unfold I; simp
+  -- }
 
   @[simp] -- I ◦ σ = σ
-  theorem subst_valid6 : r#I ⊙ σ = σ := by {
+  theorem subst_valid6 {σ : Subst Term} : I ⊙ σ = σ := by {
     funext; case _ x =>
     unfold Subst.compose; simp
     cases x
@@ -637,15 +646,15 @@ namespace Term
     case _ _ _ e => rw [e]
   }
 
-  @[simp]
-  theorem cvsubst_valid6 : cr#I ⊙ σ = σ := by {
-    funext; case _ x =>
-    unfold Subst.cvcompose; simp
-    cases x
-    all_goals (split; simp [*])
-    case _ _ _ e => rw [e]
-    case _ _ _ e => rw [e]
-  }
+  -- @[simp]
+  -- theorem cvsubst_valid6 {σ : Subst CvTerm} : I ⊙ σ = σ := by {
+  --   funext; case _ x =>
+  --   unfold Subst.cvcompose; simp
+  --   cases x
+  --   all_goals (split; simp [*])
+  --   case _ _ _ e => rw [e]
+  --   case _ _ _ e => rw [e]
+  -- }
 
   @[simp] -- (σ ◦ τ) ◦ μ = σ ◦ (τ ◦ μ)
   theorem subst_valid7 {σ : Subst Term} : σ ⊙ (τ ⊙ μ) = σ ⊙ τ ⊙ μ := by {
@@ -655,13 +664,13 @@ namespace Term
       . unfold Subst.compose; simp
   }
 
-  @[simp]
-  theorem cvsubst_valid7 {σ : Subst CvTerm} : σ ⊙ (τ ⊙ μ) = σ ⊙ τ ⊙ μ := by {
-    funext; case _ x =>
-      unfold Subst.cvcompose; simp
-      cases μ x <;> simp
-      . unfold Subst.cvcompose; simp
-  }
+  -- @[simp]
+  -- theorem cvsubst_valid7 {σ : Subst CvTerm} : σ ⊙ (τ ⊙ μ) = σ ⊙ τ ⊙ μ := by {
+  --   funext; case _ x =>
+  --     unfold Subst.cvcompose; simp
+  --     cases μ x <;> simp
+  --     . unfold Subst.cvcompose; simp
+  -- }
 
   @[simp] -- (s.σ ) ◦ τ = s[τ].(σ ◦ τ)
   theorem subst_valid8_replace {s : Term}
@@ -672,14 +681,14 @@ namespace Term
     all_goals (unfold Subst.compose; unfold Subst.cons; simp)
   }
 
-  @[simp]
-  theorem cvsubst_valid8_replace {s : CvTerm}
-    : τ ⊙ (.replace s :: σ) = .replace ([τ]s) :: (τ ⊙ σ)
-  := by {
-    funext; case _ x =>
-    cases x
-    all_goals (unfold Subst.cvcompose; unfold Subst.cons; simp)
-  }
+  -- @[simp]
+  -- theorem cvsubst_valid8_replace {s : CvTerm}
+  --   : τ ⊙ (.replace s :: σ) = .replace ([τ]s) :: (τ ⊙ σ)
+  -- := by {
+  --   funext; case _ x =>
+  --   cases x
+  --   all_goals (unfold Subst.cvcompose; unfold Subst.cons; simp)
+  -- }
 
   @[simp] -- (s.σ ) ◦ τ = s[τ].(σ ◦ τ)
   theorem subst_valid8_rename {σ : Subst Term}
@@ -690,65 +699,61 @@ namespace Term
     all_goals (unfold Subst.compose; unfold Subst.cons; simp)
   }
 
-  @[simp] -- (s.σ ) ◦ τ = s[τ].(σ ◦ τ)
-  theorem cvsubst_valid8_rename {σ : Subst CvTerm}
-    : τ ⊙ (.rename s :: σ) = (τ s) :: (τ ⊙ σ)
-  := by {
-    funext; case _ x =>
-    cases x
-    all_goals (unfold Subst.cvcompose; unfold Subst.cons; simp)
-  }
-
-  @[simp] -- S ◦ (s.σ ) = σ
-  theorem subst_valid9 : (s :: σ) ⊙ r#S = σ := by {
-    funext; case _ x =>
-    cases x
-    all_goals {
-      unfold Subst.compose; unfold Subst.cons; unfold Subst.from_ren
-      unfold S; simp
-    }
-  }
-
-  @[simp]
-  theorem cvsubst_valid9 : (s :: σ) ⊙ cr#S = σ := by {
-    funext; case _ x =>
-    cases x
-    all_goals {
-      unfold Subst.cvcompose; unfold Subst.cons; unfold Subst.from_ren
-      unfold S; simp
-    }
-  }
-
-  -- @[simp] -- 0[σ ].(S ◦ σ ) = σ
-  -- theorem subst_valid10 : .rename 0 :: r#S ⊙ σ = σ := by {
+  -- @[simp] -- (s.σ ) ◦ τ = s[τ].(σ ◦ τ)
+  -- theorem cvsubst_valid8_rename {σ : Subst CvTerm}
+  --   : τ ⊙ (.rename s :: σ) = (τ s) :: (τ ⊙ σ)
+  -- := by {
   --   funext; case _ x =>
   --   cases x
-  --   case _ => {
-  --     unfold Subst.cons; simp;
-  --     sorry
-  --   }
-  --   case _ n => {
-  --     unfold Subst.cons; simp; unfold Subst.compose; simp
-  --     unfold S; sorry
+  --   all_goals (unfold Subst.cvcompose; unfold Subst.cons; simp)
+  -- }
+
+  @[simp] -- S ◦ (s.σ ) = σ
+  theorem subst_valid9 : (s :: σ) ⊙ S = σ := by {
+    funext; case _ x =>
+    cases x
+    all_goals {
+      unfold Subst.compose; unfold Subst.cons; unfold S; simp
+    }
+  }
+
+  -- @[simp]
+  -- theorem cvsubst_valid9 : (s :: σ) ⊙ cr#S = σ := by {
+  --   funext; case _ x =>
+  --   cases x
+  --   all_goals {
+  --     unfold Subst.cvcompose; unfold Subst.cons; unfold Subst.from_ren
+  --     unfold S; simp
   --   }
   -- }
+
+  @[simp] -- 0[σ ].(S ◦ σ ) = σ
+  theorem subst_valid10 : σ 0 :: (σ ⊙ S) = σ := by {
+    funext
+    case _ x =>
+      cases x
+      case _ =>
+        simp
+      case _ =>
+        simp; unfold S; unfold Subst.compose; simp
+  }
 
   -- (βst)[σ ] = β(s[⇑σ ])(t[σ ])
   theorem subst_beta_distr : [σ](s β[t]) = ([^σ]s) β[ [σ]t ] := by simp
 
   -- s[σ ][S] = s[S][⇑σ ]
-  theorem subst_rw_ex1 : [r#S][σ]s = [^σ][r#S]s := by simp
+  theorem subst_rw_ex1 : [S][σ]s = [^σ][S]s := by simp
   -- -- s[⇑σ ][t.I] = s[t.σ ]
-  theorem subst_rw_ex2 : [t::r#I][^σ]s = [t::σ]s := by simp
+  theorem subst_rw_ex2 : [t::I][^σ]s = [t::σ]s := by simp
   -- s[⇑σ ][t[σ ].I] = s[t.I][σ ]
-  theorem subst_rw_ex3 : [(.replace ([σ]t))::r#I][^σ]s = [σ][.replace t::r#I]s := by simp
+  theorem subst_rw_ex3 : [(.replace ([σ]t))::I][^σ]s = [σ][.replace t::I]s := by simp
 
-  -- s[σ ][S] = s[S][⇑σ ]
-  theorem cvsubst_rw_ex1 : [cr#S][σ]s = [^σ][cr#S]s := by simp
-  -- -- s[⇑σ ][t.I] = s[t.σ ]
-  theorem cvsubst_rw_ex2 : [t::cr#I][^σ]s = [t::σ]s := by simp
-  -- s[⇑σ ][t[σ ].I] = s[t.I][σ ]
-  theorem cvsubst_rw_ex3 : [(.replace ([σ]t))::cr#I][^σ]s = [σ][.replace t::cr#I]s := by simp
+  -- -- s[σ ][S] = s[S][⇑σ ]
+  -- theorem cvsubst_rw_ex1 : [cr#S][σ]s = [^σ][cr#S]s := by simp
+  -- -- -- s[⇑σ ][t.I] = s[t.σ ]
+  -- theorem cvsubst_rw_ex2 : [t::cr#I][^σ]s = [t::σ]s := by simp
+  -- -- s[⇑σ ][t[σ ].I] = s[t.I][σ ]
+  -- theorem cvsubst_rw_ex3 : [(.replace ([σ]t))::cr#I][^σ]s = [σ][.replace t::cr#I]s := by simp
 
   @[simp]
   def mode_to_sort : Mode -> Const
@@ -758,17 +763,17 @@ namespace Term
 
   @[simp]
   def eta : Mode -> Term -> Term -> Term
-  | m, A, t => lam m A (app m ([r#S]t) (bound (mode_to_sort m) 0))
+  | m, A, t => lam m A (app m ([S]t) (bound (mode_to_sort m) 0))
 
   @[simp]
-  theorem S_after_Pn : (r#S ⊙ r#(Pn n)) (n + k) = .rename (k + 1) := by {
+  theorem S_after_Pn : (S ⊙ (Pn n)) (n + k) = .rename (k + 1) := by {
     cases n
     case _ => unfold Subst.compose; simp
     case _ n => unfold Subst.compose; simp; omega
   }
 
   @[simp]
-  theorem S_after_Pn_1 : (r#S ⊙ r#(Pn 1)) 1 = .rename 1 := by {
+  theorem S_after_Pn_1 : (S ⊙ (Pn 1)) 1 = .rename 1 := by {
     unfold Subst.compose; simp
   }
 
